src/lifting.v
@@ -12,7 +12,7 @@ Implicit Types (ρ : @env_state val) (σ : gmap loc val).
 Fixpoint make_stack (k : stack) : env_state * nat :=
   match k with
   | [] => (∅, O)
-  | (r, _) :: k' => let '(ρ, n) := make_stack k' in (<[n := r]>ρ, S n)
+  | r :: k' => let '(ρ, n) := make_stack k' in (<[n := r]>ρ, S n)
   end.
 
 Definition stack_depth k := snd (make_stack k).
@@ -51,23 +51,35 @@ Proof. rewrite -wp_aux.(seal_eq) //. Qed.
 Lemma wp_unfold E s Q : wp E s Q ⊣⊢ wp_pre wp E s Q.
 Proof. rewrite wp_unseal. apply (fixpoint_unfold wp_pre). Qed.
 
-Definition wp' E s Q := (∀ R, <obj> (∀ e, (wp_expr E e (λ v, Q (Some v)) -∗ wp E (Sreturn e) R)) -∗
-  (Q None -∗ R) -∗
-  wp E s R)%I.
+Lemma wp_mono E s P Q : <obj> (P -∗ Q) ⊢ wp E s P -∗ wp E s Q.
+Proof.
+  split => n; monPred.unseal.
+  iIntros "HPQ" (? <-) "H".
+  iLöb as "IH" forall (n s P Q).
+  rewrite !wp_unfold /wp_pre; monPred.unseal.
+  iDestruct "H" as "[(% & H) | H]".
+  - iLeft; iSplit => //.
+    by iApply "HPQ".
+  - iRight.
+    iIntros (???<-) "S"; iMod ("H" with "[//] S") as "H".
+    iIntros "!> %%%<- Hstack".
+    rewrite {1 3}/stack_match.
+    destruct (make_stack _) eqn: Hstack.
+    rewrite /stack_level; monPred.unseal.
+    iDestruct "Hstack" as %(<- & ?).
+    iDestruct ("H" with "[//] []") as (?????) "H".
+    { setoid_rewrite Hstack; done. }
+    iExists _, _, _, _; iSplit => //.
+    iNext; iMod "H" as (?) "($ & $ & H)".
+    iApply ("IH" with "[HPQ] H").
+    iIntros (??); iApply "HPQ".
+Qed.
 
 Lemma wp_skip E R : R ⊢ wp E skip R.
 Proof.
   iIntros "R".
   rewrite wp_unfold /wp_pre. iLeft.
   iSplit; done.
-Qed.
-
-Lemma wp'_skip E Q : Q None ⊢ wp' E skip Q.
-Proof.
-  rewrite /wp'. iIntros "? % He R".
-  rewrite wp_unfold /wp_pre. iLeft.
-  iSplit; first done.
-  iApply "R". done.
 Qed.
 
 Lemma var_e : forall x v σ ρ r k,
@@ -112,34 +124,235 @@ Proof.
   iIntros "(#? & %) P"; iApply stack_level_embed; by iFrame "# ∗".
 Qed.
 
-Definition get_params f := let 'Func params _ _ := f in params.
-Definition get_locals f := let 'Func _ locals _ := f in locals.
-Definition get_body f := let 'Func _ _ body := f in body.
+Lemma wp_seq E s1 s2 Q : wp E s1 (▷ wp E s2 Q) ⊢ wp E (Sseq s1 s2) Q.
+Proof.
+  split => n.
+  iIntros "H".
+  iLöb as "IH" forall (s1 s2 Q n).
+  rewrite wp_unfold [wp _ (s1;;s2)%S _]wp_unfold /wp_pre.
+  monPred.unseal.
+  iRight.
+  iIntros (???<-) "S".
+  iDestruct "H" as "[[-> >Hs1] | H]".
+  - iApply fupd_mask_intro; first set_solver; iIntros "Hclose" (???<-) "Hstack".
+    iExists _, _, _, _. iSplit.
+    { iPureIntro. apply SeqS2. }
+    { iNext; iFrame.
+      rewrite /stack_match /stack_depth.
+      destruct (make_stack x2).
+      rewrite /stack_level; monPred.unseal.
+      iDestruct "Hstack" as (<-) "$".
+      iMod "Hclose". iModIntro; iSplit => //.
+    }
+  - iDestruct ("H" with "[//] [$]") as ">H".
+    iModIntro.
+    iIntros (r k ? <-) "Hmatch".
+    iDestruct ("H" with "[//] [$Hmatch]") as (????) "(% & H)".
+    iExists _, _, _, _.
+    iSplit; first by (iPureIntro; econstructor).
+    clear.
+    iNext; iMod "H" as (ρ) "($ & ? & ?)"; iModIntro.
+    rewrite -monPred_at_sep.
+    iApply (stack_match_stack_depth with "[$] [-]").
+    iApply "IH"; iFrame.
+Qed.
 
-Definition stack_size f := let 'Func params locals _ := f in
+Definition get_params f := let 'Func params _ _ _ := f in params.
+Definition get_locals f := let 'Func _ locals _ _ := f in locals.
+Definition get_body f := let 'Func _ _ body _ := f in body.
+Definition get_ret f := let 'Func _ _ _ e := f in e.
+
+Definition stack_size f := let 'Func params locals _ _ := f in
   (length params + length locals)%nat.
 
 Definition stack_frac f := (/ pos_to_Qp (Pos.of_nat (1 + stack_size f)))%Qp.
 
-Definition stack_retainer f := assert_of (λ n,
-  stack_frag n (stack_frac f) (stack_frac f) ∅).
+Definition stack_retainer f := (∃ n, stack_level (S n) ∗ ⎡stack_frag (S n) (stack_frac f) (stack_frac f) ∅⎤)%I.
 
 Definition stackframe f vs := ([∗ list] x;v ∈ (get_params f ++ get_locals f);vs, points_to_var x v)%I.
 
 Definition call_assert E f vs x R := (⇑ (stack_retainer f -∗ stackframe f vs -∗
-  wp' E (get_body f) ((λ v', ∃ v, ⌜Some v = v'⌝ ∧ stack_retainer f ∗
+  wp E (get_body f) (wp_expr E (get_ret f) (λ v, stack_retainer f ∗
     (∃ vs, ⌜stack_size f = length vs⌝ ∧ stackframe f vs) ∗
     ⇓ ((∃ v, points_to_var x v) ∗ ▷ (points_to_var x v -∗ R))))))%I.
 
-Lemma wp_return E e Q : wp_expr E e (λ v, Q $ Some v) ⊢ wp' E (Sreturn e) Q.
+Lemma wp_exprs_app E es Q σ ρ : wp_exprs E es Q -∗ ⎡state_interp σ ρ⎤ ={E}=∗
+  ∃ vs, (∀ r k, env_match ρ r -∗ ⌜eval_exprs' es (Build_state r σ k) vs⌝) ∗ ⎡state_interp σ ρ⎤ ∗ Q vs.
 Proof.
-  iIntros "H % Hret R". rewrite monPred_objectively_elim; by iApply "Hret".
+  iIntros "Hes S"; iInduction es as [|e es] "IH" forall (Q); simpl.
+  - iFrame. iIntros "!> %% ?"; iPureIntro; constructor.
+  - rewrite /wp_expr.
+    iMod ("Hes" with "S") as (?) "(He & S & Hes)".
+    iMod ("IH" with "Hes S") as (?) "(Hes & $ & $)".
+    iIntros "!> %% Henv".
+    iDestruct ("He" with "Henv") as %?; iDestruct ("Hes" $! _ k with "Henv") as %?.
+    iPureIntro; by constructor.
+Qed.
+
+Lemma stack_depth_max : forall k ρ n, make_stack k = (ρ, n) → ∀ m, n ≤ m → ρ !! m = None.
+Proof.
+  induction k; simpl; try done.
+  - inversion 1; intros; by rewrite lookup_empty.
+  - destruct (make_stack k) eqn: Hk; inversion 1; subst; intros.
+    rewrite lookup_insert_ne; last lia.
+    eapply IHk; eauto; lia.
+Qed.
+
+Lemma add_frame σ ρ r k xs vs : ⎡state_interp σ ρ⎤ ∗ stack_match ρ r k ⊢
+  |==> ∃ ρ', ⎡state_interp σ ρ'⎤ ∗ ⇑ (stack_match ρ' (bind_vars xs vs) (r :: k) ∗
+    assert_of (λ n, stack_frag n (/ pos_to_Qp (Pos.of_nat (1 + size (bind_vars xs vs))))%Qp 1%Qp (bind_vars xs vs))).
+Proof.
+  intros; rewrite /stack_match /=.
+  destruct (make_stack k) eqn: Hk.
+  iIntros "(Hρ & #Hl & ->)".
+  iMod (state_interp_alloc_frame _ _ (S n) with "Hρ") as "($ & ?)".
+  { rewrite lookup_insert_ne //.
+    eapply stack_depth_max; eauto. }
+  iModIntro.
+  rewrite -!up1_sep.
+  iPoseProof (stack_level_up with "Hl") as "$".
+  rewrite -up1_objective; iSplit; first done.
+  iStopProof; split => ?; rewrite /stack_level; monPred.unseal; rewrite monPred_at_intuitionistically /=.
+  iIntros "((<- & _) & $)".
+Qed.
+
+Lemma pure_sep_equiv P (Q R : iProp Σ) : (P → (Q ⊣⊢ R)) → ⌜P⌝ ∗ Q ⊣⊢ ⌜P⌝ ∗ R.
+Proof.
+  intros; iSplit; iIntros "(% & ?)"; iSplit => //.
+  - rewrite H //.
+  - rewrite -H //.
+Qed.
+
+Lemma split_stackframe params locals body e vs :
+  length (params ++ locals) = length vs → NoDup (params ++ locals) →
+  let r' := bind_vars (params ++ locals) vs in
+  (∃ n, stack_level (S n) ∗ assert_of (λ n, stack_frag n (/ pos_to_Qp (Pos.of_nat (1 + size r')))%Qp 1%Qp r')) ⊣⊢
+  stack_retainer (Func params locals body e) ∗ stackframe (Func params locals body e) vs.
+Proof.
+  split => n /=; rewrite /stack_retainer /stackframe /stack_level; monPred.unseal.
+  rewrite bi.sep_exist_r; do 2 f_equiv.
+  rewrite -assoc; apply pure_sep_equiv; intros [=]; subst.
+  rewrite monPred_at_big_sepL2 vars_equiv //.
+  case_decide.
+  - destruct params; last done; destruct locals; last done; rewrite /bind_vars /stack_frac /= bi.sep_emp.
+    by rewrite map_size_empty Qp.inv_1.
+  - rewrite /stack_frac /=.
+    replace (size _) with (length (params ++ locals)).
+    rewrite -app_length.
+    iSplit.
+    + rewrite Nat2Pos.inj_succ // Pplus_one_succ_l -pos_to_Qp_add.
+      set (q := (1 + _)%Qp).
+      rewrite -(Qp.mul_inv_r q).
+      destruct (q - 1)%Qp eqn: Hq.
+      apply Qp.sub_Some in Hq; rewrite {2} Hq Qp.mul_add_distr_r -frac_op.
+      rewrite -{1}(map_empty_union (bind_vars _ _)) stack_frag_split.
+      rewrite Qp.mul_1_l; iIntros "($ & ?)".
+      iExists _; iStopProof; f_equiv; try done.
+      * apply Qp.add_inj_r in Hq as <-; done.
+      * apply map_disjoint_empty_l.
+      * by apply Qp.sub_None, Qp.not_add_le_l in Hq.
+    + iIntros "(Hret & % & H)".
+      iDestruct (stack_frag_join with "[$Hret $H]") as ((<- & _)) "H".
+      rewrite !left_id Nat2Pos.inj_succ // Pplus_one_succ_l -pos_to_Qp_add.
+      set (q := (1 + _)%Qp).
+      by rewrite -{2}(Qp.mul_1_l (/ q)) -Qp.mul_add_distr_r Qp.mul_inv_r.
+    + rewrite map_size_list_to_map; last by rewrite fst_zip; try lia.
+      rewrite length_zip_with_l_eq //.
+Qed.
+
+Lemma remove_frame σ ρ r r0 k q r' : ⎡state_interp σ ρ⎤ ∗ stack_match ρ r (r0 :: k) ∗ assert_of (λ n, stack_frag n q 1%Qp r') ⊢
+  |==> ∃ ρ', ⎡state_interp σ ρ'⎤ ∗ ⇓ stack_match ρ' r0 k.
+Proof.
+  intros; rewrite /stack_match /=.
+  destruct (make_stack k) eqn: Hk.
+  iIntros "(Hρ & (#Hl & ->) & H)".
+  iMod (state_interp_dealloc_frame _ _ (S n) with "[$Hρ H]") as "$".
+  { iApply (stack_level_embed with "Hl H"). }
+  iModIntro.
+  rewrite -!down1_sep.
+  iPoseProof (stack_level_down with "Hl") as "$".
+  rewrite -down1_objective; iPureIntro.
+  apply (delete_insert _ _ r).
+  rewrite lookup_insert_ne //; eapply stack_depth_max; eauto.
+Qed.
+
+Lemma wp_call E x f es Q : wp_exprs E es (λ vs, ∃ fd, ⌜F !! f = Some fd ∧
+    length es = length (get_params fd) ∧ NoDup (get_params fd ++ get_locals fd)⌝ ∧
+  ▷ call_assert E fd (vs ++ repeat (NumV 0) (length (get_locals fd))) x Q) ⊢
+  wp E (Scall x f es) Q.
+Proof.
+  iIntros "H".
+  rewrite wp_unfold /wp_pre; iRight.
+  iIntros (??) "S".
+  iMod (wp_exprs_app with "H S") as (?) "(Hes & S & %fd & (% & %Hlen & %) & H)".
+  destruct fd; simpl in *.
+  iApply fupd_mask_intro; first set_solver; iIntros "Hclose" (??) "Hstack".
+  iDestruct ("Hes" with "[Hstack]") as %?; first by iApply stack_env_match.
+  iExists _, _, _, _; iSplit.
+  { iPureIntro; by econstructor. }
+  iNext.
+  iMod (add_frame with "[$S $Hstack]") as (?) "($ & Hstack)".
+  iMod "Hclose" as "_"; iModIntro; simpl.
+  iApply up1_obj_elim; iApply up1_mono; last first.
+  { rewrite /call_assert.
+    iCombine "H Hstack" as "H"; rewrite !up1_sep; iApply "H". }
+  iIntros "(H & Hstack & Hframe)".
+  iAssert (stack_level (S (stack_depth k))) with "[Hstack]" as "#Hl".
+  { rewrite /stack_match /stack_depth /=. destruct (make_stack k); iDestruct "Hstack" as "($ & _)". }
+  iApply (stack_match_embed with "Hstack").
+  assert (length (func_params ++ func_locals) = length (vs ++ repeat (NumV 0) (length func_locals))).
+  { rewrite !app_length repeat_length; f_equal.
+    rewrite -Hlen; by eapply Forall2_length. }
+  iPoseProof (bi.equiv_entails_1_1 with "[Hframe]") as "Hframe"; first by apply split_stackframe.
+  { iFrame; eauto. }
+  iDestruct "Hframe" as "(Hret & Hframe)".
+  iApply wp_seq. iApply wp_mono; last by iApply ("H" with "Hret Hframe").
+  rewrite monPred_objectively_unfold; iIntros "!>" (?); monPred.unseal.
+  iIntros (??) "H !>".
+  rewrite wp_unfold /wp_pre /wp_expr; monPred.unseal.
+  iRight; iStopProof; do 8 f_equiv.
+  iIntros ">(% & He & (Hσ & Hρ) & Hret & Hframe & (% & Hx) & H)".
+  iDestruct (stack_ra.var_e with "[$Hx $Hρ]") as %?.
+  iApply fupd_mask_intro; first set_solver; iIntros "Hclose" (???<-) "Hstack".
+  rewrite {1}/stack_match.
+  destruct (make_stack _) eqn: Hstack.
+  rewrite /stack_level; monPred.unseal.
+  iDestruct "Hstack" as %([=] & ->).
+  rewrite /stack_retainer /stack_level; monPred.unseal.
+  iDestruct "Hret" as (? [=]) "Hret"; subst; simpl in *.
+  iDestruct ("He" with "[//] []") as %?.
+  { by rewrite lookup_insert. }
+  destruct x3; try done.
+  iExists _,_, _, _; iSplit.
+  { iPureIntro; by econstructor. }
+  iNext.
+  iDestruct "Hframe" as (??) "Hframe".
+  iPoseProof (monPred_in_entails with "[Hσ Hρ Hret Hframe]") as "H'"; first apply remove_frame.
+  { monPred.unseal; iFrame.
+    iAssert (stack_retainer (Func func_params func_locals func_body func_ret) (S x4)) with "[Hret]" as "Hret".
+    { rewrite /stack_retainer /stack_level; monPred.unseal; by iFrame. }
+    iCombine "Hret Hframe" as "H".
+    rewrite -monPred_at_sep monPred_in_equiv; last by symmetry; apply split_stackframe; rewrite ?app_length.
+    monPred.unseal; iDestruct "H" as (?) "(_ & $)".
+    rewrite /stack_match /stack_level; setoid_rewrite Hstack; by monPred.unseal. }
+  monPred.unseal; iMod "H'" as (?) "(S & Hstack)".
+  iPoseProof (monPred_in_entails with "[S Hstack Hx]") as "H'"; first apply var_update.
+  { monPred.unseal; iFrame. }
+  monPred.unseal; iMod "H'" as (?) "(Hstack & Hx & $)".
+  iMod "Hclose"; iModIntro.
+  iSplitR "H Hx".
+  - rewrite /stack_match /stack_depth; destruct (make_stack x3); monPred.unseal.
+    iDestruct "Hstack" as "(_ & $)"; rewrite /stack_level; by monPred.unseal.
+  - simpl in Hstack.
+    rewrite /stack_depth; destruct (make_stack _).
+    inv Hstack.
+    rewrite -wp_skip; by iApply "H".
 Qed.
 
 Lemma wp_assign E x e Q : wp_expr E e (λ v, (∃ v0, x ↦v v0) ∗
-  ▷ (x ↦v v -∗ Q None)) ⊢ wp' E (Sassign x e) Q.
+  ▷ (x ↦v v -∗ Q)) ⊢ wp E (Sassign x e) Q.
 Proof.
-  iIntros "H % Hret R".
+  iIntros "H".
   rewrite wp_unfold /wp_pre /stack_depth. iRight.
   iIntros (??) "S".
   rewrite /wp_expr.
@@ -154,13 +367,13 @@ Proof.
   iMod "Hclose"; iModIntro.
   simpl.
   iApply (stack_match_embed with "[$]").
-  rewrite -wp_skip. iApply "R". iApply "Hpost". done.
+  rewrite -wp_skip. by iApply "Hpost".
 Qed.
 
 Lemma wp_alloc E x Q : (∃ v0, x ↦v v0) ∗
-  ▷ (∀ l, points_to_var x (LocV l) -∗ l ↦ NumV 0 -∗ Q None) ⊢ wp' E (Salloc x) Q.
+  ▷ (∀ l, points_to_var x (LocV l) -∗ l ↦ NumV 0 -∗ Q) ⊢ wp E (Salloc x) Q.
 Proof.
-  iIntros "H % Hret R".
+  iIntros "H".
   rewrite wp_unfold /wp_pre. iRight.
   iIntros (??) "S".
   iDestruct "H" as "((% & Hx) & Hpost)".
@@ -174,13 +387,13 @@ Proof.
   { apply next_loc_new. }
   iMod "Hclose"; iModIntro.
   iApply (stack_match_embed with "[$]").
-  rewrite -wp_skip. iApply "R". by iApply ("Hpost" with "[$]").
+  rewrite -wp_skip. by iApply ("Hpost" with "[$]").
 Qed.
 
 Lemma wp_store E e1 e2 Q : wp_expr E e2 (λ v, wp_expr E e1 (λ v1, ∃ l v0, ⌜v1 = LocV l⌝ ∧
-  l ↦ v0 ∗ ▷ (l ↦ v -∗ Q None))) ⊢ wp' E (Sstore e1 e2) Q.
+  l ↦ v0 ∗ ▷ (l ↦ v -∗ Q))) ⊢ wp E (Sstore e1 e2) Q.
 Proof.
-  iIntros "H % Hret R".
+  iIntros "H".
   rewrite wp_unfold /wp_pre. iRight.
   iIntros (??) "S".
   rewrite /wp_expr.
@@ -196,50 +409,13 @@ Proof.
   iMod (state_interp_store with "S Hl") as "($ & ?)"; iFrame.
   iMod "Hclose"; iModIntro.
   iApply (stack_match_embed with "[$]").
-  rewrite -wp_skip. iApply "R". by iApply "Hpost".
+  rewrite -wp_skip. by iApply "Hpost".
 Qed.
 
-Lemma wp_seq E s1 s2 Q : wp E s1 (▷ wp' E s2 Q) ⊢ wp' E (Sseq s1 s2) Q.
-Admitted.
-(*Proof.
-  iIntros "H % Hret R".
-  rewrite {1}/wp'; iStopProof.
-  split => i.
-  iIntros "H".
-  iLöb as "IH" forall (s1 s2 Q i).
-  rewrite wp_unfold [wp _ (s1;;s2)%S _]wp_unfold /wp_pre.
-  monPred.unseal.
-  iDestruct "H" as "(H & Hret)".
-  iRight.
-  iIntros (???<-) "S".
-  iDestruct "H" as "[[-> >Hs1] | H]".
-  - iApply fupd_mask_intro; first set_solver; iIntros "Hclose" (???<-) "Hstack".
-   iExists _, _, _, _. iSplit.
-    { iPureIntro. apply SeqS2. }
-    { iNext; iFrame.
-      destruct (make_stack x2).
-      iMod "Hclose". iModIntro.
-      iSpecialize ("Hs1" with "[//] Hret").
-      rewrite -monPred_at_sep.
-      iApply (stack_match_stack_depth with "[$] [$]").
-    }
-  - iDestruct ("H" with "[//] [$]") as ">H".
-    iModIntro.
-    iIntros (r k ? <-) "Hmatch".
-    iDestruct ("H" with "[//] [$Hmatch]") as (????) "(% & H)".
-    iExists _, _, _, _.
-    iSplit; first by (iPureIntro; econstructor).
-    clear.
-    iNext; iMod "H" as (ρ) "($ & ? & ?)"; iModIntro.
-    rewrite -monPred_at_sep.
-    iApply (stack_match_stack_depth with "[$] [-]").
-    iApply "IH"; iFrame.
-Qed. *)
-
 Lemma wp_if E e s1 s2 Q : wp_expr E e (λ v, ∃ n, ⌜v = NumV n⌝ ∧
-  ▷ wp' E (if Z.eqb n 0 then s2 else s1) Q) ⊢ wp' E (Sif e s1 s2) Q.
+  ▷ wp E (if Z.eqb n 0 then s2 else s1) Q) ⊢ wp E (Sif e s1 s2) Q.
 Proof.
-  iIntros "H % Hret R".
+  iIntros "H".
   rewrite wp_unfold /wp_pre. iRight.
   iIntros (??) "S".
   rewrite /wp_expr.
@@ -250,15 +426,15 @@ Proof.
   { iPureIntro; by econstructor. }
   iNext; iFrame.
   iApply (stack_match_embed with "[$]").
-  iMod "Hclose". iApply ("H" with "[$] [$]").
+  iMod "Hclose". iApply "H".
 Qed.
 
 Lemma wp_while E e s Q : wp_expr E e (λ v, ∃ n, ⌜v = NumV n⌝ ∧
-  ▷ if Z.eqb n 0 then Q None else wp' E s (λ _, ▷ wp' E (Swhile e s) Q)) ⊢
-  wp' E (Swhile e s) Q.
+  ▷ if Z.eqb n 0 then Q else wp E s (▷ wp E (Swhile e s) Q)) ⊢
+  wp E (Swhile e s) Q.
 Proof.
-  iIntros "H % Hret R".
-  rewrite wp_unfold /wp_pre. iRight.
+  iIntros "H".
+  rewrite {2}[wp _ (Swhile _ _) _]wp_unfold /wp_pre. iRight.
   iIntros (??) "S".
   rewrite /wp_expr.
   iMod ("H" with "S") as (?) "(He & S & % & -> & H)".
@@ -270,16 +446,14 @@ Proof.
     iNext; iFrame.
     iMod "Hclose" as "_"; iModIntro.
     rewrite Heqb -wp_skip //.
-    iApply (stack_match_embed with "[$]").
-    by iApply "R".
+    by iApply (stack_match_embed with "[$]").
   - iExists _, _, _, _; iSplit.
     { iPureIntro; econstructor; eauto. }
     iNext; iFrame.
     iMod "Hclose" as "_"; iModIntro.
-    (* rewrite Heqb -wp_seq //.
-    by iApply (stack_match_embed with "[$]"). *)
-Admitted.
-
+    rewrite Heqb -wp_seq //.
+    by iApply (stack_match_embed with "[$]").
+Qed.
 
 End wp.
 
@@ -358,7 +532,7 @@ Qed.
 
 Lemma wp_adequacy Σ `{!gen_heapGpreS loc val Σ} `{!inG Σ (@envR val)} `{!invGpreS Σ} F s σ φ :
   (∀ `{!gen_heapGS loc val Σ} `{!envGS val Σ} `{Hinv : !invGS_gen HasNoLc Σ},
-     ⊢ |={⊤}=> wp' F ⊤ s (λ v, ⌜v = None ∧ φ⌝)) →
+     ⊢ |={⊤}=> wp F ⊤ s (⌜φ⌝)) →
   adequate F s (Build_state ∅ σ []) (λ _, φ).
 Proof.
   intros Hwp. apply adequate_alt; intros s2 σ2 H.
@@ -371,23 +545,6 @@ Proof.
   iPoseProof (monPred_in_entails _ _ (Hwp _ _ _) O with "[]") as "Hwp"; clear Hwp.
   { by monPred.unseal. }
   rewrite monPred_at_fupd; iMod "Hwp".
-  rewrite /wp'.
-  remember (λ v : val, _) as Φ.
-  monPred.unseal.
-  iSpecialize ("Hwp" $! ⌜φ⌝%I with "[//] [] [//] []").
-  2: { by iIntros (?? (? & ?)); monPred.unseal. }
-  { iIntros (???[=]). iApply monPred_in_entails. iIntros "H".
-    rewrite wp_unfold /wp_pre /wp_expr.
-    iRight. iIntros (??) "S".
-    iMod ("H" with "S") as "(%v & Hv & S & HΦ)".
-    iApply fupd_mask_intro; first set_solver.
-    iIntros "Hclose" (??) "stack".
-    iPoseProof ("Hv" $! r with "[-]") as "%".
-    { by iApply stack_env_match. }
-    subst.
-    iDestruct "HΦ" as %(? & ?); done.
-  }
-
   iAssert (stack_match {[0 := ∅]} ∅ [] O) as "-#Hstack".
   { rewrite /stack_match /stack_level; by monPred.unseal. }
 
@@ -397,7 +554,6 @@ Proof.
   set (l := 0); clearbody l.
   iInduction n as [|n] "IH" forall (σ ρ r k l s H).
   - inv H.
-    rewrite /wp'.
      rewrite wp_unfold /wp_pre; monPred.unseal.
     iDestruct "Hwp" as "[Hwp | Hwp]".
     + iDestruct "Hwp" as "(-> & >%)".
